(try and fail to) derive alt specs from base ones

rocq-brick-libstdcpp/proof/mutex/spec/unique_lock.v
@@ -57,13 +57,19 @@ Section with_cpp.
       Definition do_unlock (thr : thread_idT) (lk : ptr * gname * Qp * mpred) (Q : mpred) : mpred :=
         match lk with
         | (mp, g, q, P) =>
-          mutex.locked g thr q ** ▷P ** ▷(mutex.token g q -* Q)
+          mutex.locked g thr q ** ▷P **
+          (* TODO readd *)
+          (* ▷ *)
+          (mutex.token g q -* Q)
         end.
 
       Definition do_lock (thr : thread_idT) (lk : ptr * gname * Qp * mpred) (Q : mpred) : mpred :=
         match lk with
         | (mp, g, q, P) =>
-          mutex.token g q ** ▷(mutex.locked g thr q ** ▷P -* Q)
+          mutex.token g q **
+          (* TODO readd *)
+          (* ▷ *)
+          (mutex.locked g thr q ** ▷P -* Q)
         end.
 
       cpp.spec "std::unique_lock<std::mutex>::unique_lock()"
@@ -243,6 +249,46 @@ Section with_cpp.
           this |-> R 1$m (Some (false, mm)) **
           K
       ).
+
+      Lemma lock_spec_entails_lock_spec_alt : lock_spec |-- lock_spec_alt.
+      Proof.
+        apply specify_mono.
+        rewrite /do_lock.
+        go.
+        (* XXX needs removing later in do_lock, or a stronger specify_mono offering a later. *)
+        repeat case_match; go.
+      Qed.
+
+      Lemma unlock_spec_entails_unlock_spec_alt : unlock_spec |-- unlock_spec_alt.
+      Proof.
+        apply specify_mono.
+        rewrite /do_unlock.
+        go.
+        (* XXX needs removing later in do_unlock, or a stronger specify_mono offering a later. *)
+        repeat case_match; go.
+      Qed.
+
+      Lemma lock_spec_alt_entails_lock_spec : lock_spec_alt |-- lock_spec.
+      Proof.
+        apply specify_mono.
+        rewrite /do_lock.
+        go.
+        iExists (mutex.locked g thr q ∗ ▷ P)%I.
+        go.
+        (* failed goal: ▷ P -∗ P. This might work with a stronger specify_mono offering a later. *)
+        admit.
+        all: fail.
+      Abort.
+
+      Lemma unlock_spec_alt_entails_unlock_spec : unlock_spec_alt |-- unlock_spec.
+      Proof.
+        apply specify_mono.
+        rewrite /do_unlock.
+        go.
+        iExists (mutex.token g q).
+        go.
+      Qed.
+
     End with_threads.
 End with_cpp.
 End unique_lock.
